GCM.v
@@ -1,0 +1,196 @@
+Set Implicit Arguments.
+
+Require Import FPUtil.
+
+Require Import AES.
+
+Require Import Arith NArith NPeano Ascii String List.
+Import ListNotations.
+Open Scope N_scope.
+Open Scope nat_scope.
+Open Scope string_scope.
+Open Scope list_scope.
+Open Scope bitvec_scope.
+
+Section GCM.
+
+  Definition stateful_map S (upd : S -> S) (init : S) A (f : A -> S -> A) (ls : list A) : list A * S :=
+    let step (p : list A * S) x :=
+        let (acc, st) := p in
+        let y := f x st in
+        (y :: acc, upd st) in
+    let (ls, final) := fold_left step ls ([], init) in
+    (rev ls, final).
+
+  Definition fold_left_i A B (f : nat -> A -> B -> A) (ls : list B) init init_i :=
+    fst $ fold_left (fun (p : A * nat) x => let (a, i) := p in (f i a x, S i)) ls (init, init_i).
+
+  Definition len A := @length A >> msb_of_nat 64.
+
+  Infix "=?" := beq_nat : nat_scope.
+
+  Definition gf128_mul := gf_mul 128 "11100001".
+
+  Infix "*" := gf128_mul : bitvec_scope.
+  Infix "+" := xor : bitvec_scope.
+
+  Definition GHASH (H : b128) (A : bitvec) (C : bitvec) : bitvec :=
+    let As := slice 128 A in
+    let Cs := slice 128 C in
+    let m := length As in
+    let n := length Cs in
+    let step i (X Y : b128) :=
+        let Y := if (i =? m - 1) || (i =? m + n - 1) then
+                   right_trunc_pad_to 128 Y
+                 else
+                   Y in
+        (X + Y) * H in
+    let X := fold_left_i step (As ++ Cs) (zeros 128) 0 in
+    (X + (len A ++ len C)) * H.
+
+  Variable E : key_t -> b128 -> b128. 
+  Variable K : key_t.
+  Definition IV_t := bitvec.
+  Variable IV : IV_t.
+  Variable P : bitvec.
+  Definition A_t := bitvec.
+  Variable A : A_t.
+  Variable t : nat.
+
+  Definition H := E K $ zeros 128.
+
+  Definition msb_unsign_plus (a b : bitvec) : bitvec := msb_of_nat (length a) ((msb_to_nat a) + (msb_to_nat b)).
+
+  Definition incr v := 
+    let F_len := length v - 32 in
+    let F := firstn F_len v in
+    let I := skipn F_len v in
+    F ++ (msb_unsign_plus I (msb_of_nat 32 1)).
+
+  Definition Y0 :=
+    if length IV =? 96 then
+      IV ++ zeros 31 ++ bin "1"
+    else
+      GHASH H [] IV.
+
+  Definition C : bitvec :=
+    match P with
+      | nil => nil
+      | _ =>
+        let Ps := slice 128 P in
+        let Pi := removelast Ps in
+        let Pn := last Ps (zeros 128) in
+        let (Ci, Yn) := stateful_map incr (incr Y0) (fun Pi Yi => Pi + E K Yi) Pi in
+        let Cn := Pn + firstn (length Pn) (E K Yn) in
+        flat Ci ++ Cn
+    end.
+
+  Definition T := firstn t $ GHASH H A C + E K Y0.
+
+  Definition encrypt := (C, T).
+
+End GCM.
+
+Notation E := AES.encrypt.
+
+Module test1.
+  Definition t_K := hex "00000000000000000000000000000000".
+  Definition t_P := hex "".
+  Definition t_IV := hex "000000000000000000000000".
+  Definition t_H := hex "66e94bd4ef8a2c3b884cfa59ca342b2e".
+  Goal (H E t_K) = t_H. r. Qed.
+  Definition t_Y0 := hex "00000000000000000000000000000001".
+  Goal (Y0 E t_K t_IV) = t_Y0. r. Qed.
+  Definition t_E_K_Y0 := hex "58e2fccefa7e3061367f1d57a4e7455a".
+  Goal E t_K t_Y0 = t_E_K_Y0. r. Qed.
+  Definition t_C := hex "".
+  Goal (C E t_K t_IV t_P) = t_C. r. Qed.
+  Definition t_lenA_lenC := hex "00000000000000000000000000000000".
+  Definition t_A := hex "".
+  Goal len t_A ++ len t_C = t_lenA_lenC. r. Qed.
+  Definition t_GHASH := hex "00000000000000000000000000000000".
+  Goal GHASH t_H t_A t_C = t_GHASH. r. Qed.
+  Definition t_T := hex "58e2fccefa7e3061367f1d57a4e7455a".
+  Definition t_t := 128.
+  Goal T E t_K t_IV t_P t_A t_t = t_T. r. Qed.
+End test1.
+
+Module test2.
+  Definition t_K := hex "00000000000000000000000000000000".
+  Definition t_P := hex "00000000000000000000000000000000".
+  Definition t_IV := hex "000000000000000000000000".
+  Definition t_H := hex "66e94bd4ef8a2c3b884cfa59ca342b2e".
+  Goal (H E t_K) = t_H. r. Qed.
+  Definition t_Y0 := hex "00000000000000000000000000000001".
+  Goal (Y0 E t_K t_IV) = t_Y0. r. Qed.
+  Definition t_E_K_Y0 := hex "58e2fccefa7e3061367f1d57a4e7455a".
+  Goal E t_K t_Y0 = t_E_K_Y0. r. Qed.
+  Definition t_C := hex "0388dace60b6a392f328c2b971b2fe78".
+  Goal (C E t_K t_IV t_P) = t_C. r. Qed.
+  Definition t_lenA_lenC := hex "00000000000000000000000000000080".
+  Definition t_A := hex "".
+  Goal len t_A ++ len t_C = t_lenA_lenC. r. Qed.
+  Definition t_GHASH := hex "f38cbb1ad69223dcc3457ae5b6b0f885".
+  Goal GHASH t_H t_A t_C = t_GHASH. r. Qed.
+  Definition t_T := hex "ab6e47d42cec13bdf53a67b21257bddf".
+  Definition t_t := 128.
+  Goal T E t_K t_IV t_P t_A t_t = t_T. r. Qed.
+End test2.
+
+Module test3.
+  Definition t_K := hex "feffe9928665731c6d6a8f9467308308".
+  Definition t_P := flat $ map hex ["d9313225f88406e5a55909c5aff5269a";
+                                     "86a7a9531534f7da2e4c303d8a318a72";
+                                     "1c3c0c95956809532fcf0e2449a6b525";
+                                     "b16aedf5aa0de657ba637b391aafd255"].
+  Definition t_IV := hex "cafebabefacedbaddecaf888".
+  Definition t_H := hex "b83b533708bf535d0aa6e52980d53b78".
+  Goal (H E t_K) = t_H. r. Qed.
+  Definition t_Y0 := hex "cafebabefacedbaddecaf88800000001".
+  Goal (Y0 E t_K t_IV) = t_Y0. r. Qed.
+  Definition t_E_K_Y0 := hex "3247184b3c4f69a44dbcd22887bbb418".
+  Goal E t_K t_Y0 = t_E_K_Y0. r. Qed.
+  Definition t_C := flat $ map hex ["42831ec2217774244b7221b784d0d49c";
+                                     "e3aa212f2c02a4e035c17e2329aca12e";
+                                     "21d514b25466931c7d8f6a5aac84aa05";
+                                     "1ba30b396a0aac973d58e091473f5985"].
+  Goal (C E t_K t_IV t_P) = t_C. r. Qed.
+  Definition t_lenA_lenC := hex "00000000000000000000000000000200".
+  Definition t_A := hex "".
+  Goal len t_A ++ len t_C = t_lenA_lenC. r. Qed.
+  Definition t_GHASH := hex "7f1b32b81b820d02614f8895ac1d4eac".
+  Goal GHASH t_H t_A t_C = t_GHASH. r. Qed.
+  Definition t_T := hex "4d5c2af327cd64a62cf35abd2ba6fab4".
+  Definition t_t := 128.
+  Goal T E t_K t_IV t_P t_A t_t = t_T. r. Qed.
+End test3.
+
+Module test4.
+  Definition t_K := hex "feffe9928665731c6d6a8f9467308308".
+  Definition t_P := flat $ map hex ["d9313225f88406e5a55909c5aff5269a";
+                                     "86a7a9531534f7da2e4c303d8a318a72";
+                                     "1c3c0c95956809532fcf0e2449a6b525";
+                                     "b16aedf5aa0de657ba637b39"].
+  Definition t_A := flat $ map hex ["feedfacedeadbeeffeedfacedeadbeef";
+                                     "abaddad2"].
+  Definition t_IV := hex "cafebabefacedbaddecaf888".
+  Definition t_H := hex "b83b533708bf535d0aa6e52980d53b78".
+  Goal (H E t_K) = t_H. r. Qed.
+  Definition t_Y0 := hex "cafebabefacedbaddecaf88800000001".
+  Goal (Y0 E t_K t_IV) = t_Y0. r. Qed.
+  Definition t_E_K_Y0 := hex "3247184b3c4f69a44dbcd22887bbb418".
+  Goal E t_K t_Y0 = t_E_K_Y0. r. Qed.
+  Definition t_C := flat $ map hex ["42831ec2217774244b7221b784d0d49c";
+                                     "e3aa212f2c02a4e035c17e2329aca12e";
+                                     "21d514b25466931c7d8f6a5aac84aa05";
+                                     "1ba30b396a0aac973d58e091"].
+  Goal (C E t_K t_IV t_P) = t_C. r. Qed.
+  Definition t_lenA_lenC := hex "00000000000000a000000000000001e0".
+  Goal len t_A ++ len t_C = t_lenA_lenC. r. Qed.
+  Definition t_GHASH := hex "698e57f70e6ecc7fd9463b7260a9ae5f".
+  Goal GHASH t_H t_A t_C = t_GHASH. r. Qed.
+  Definition t_T := hex "5bc94fbc3221a5db94fae95ae7121a47".
+  Definition t_t := 128.
+  Goal T E t_K t_IV t_P t_A t_t = t_T. r. Qed.
+End test4.
+
